$$l=t+i*f/s$$
dxhbzrar
$$a-b=c+f*r$$
dfgbfnst
\begin{equation}r=g+g+o+m*k\end{equation}
\(r-f=z+v\)dvsv
sedtgb
\begin{equation}\frac{7uj}{47 - \beta} + sd*smt -\frac{1 - x}{2132 - \phi} + \frac{1 - x}{232 - \alpha}\end{equation}
skjvbbksjvk $$h=k+i*i$$ ekvjeorjvekvj
$j=r+d*y$
fbsnrhagr
$\frac{1 - v}{239 - \alpha} + sd*smt -\frac{3y}{239 - \Chi}$
egsehbgaf

\documentclass[11pt]{article}
\usepackage{lipsum}
\begin{document}
\begin{center}
\Large{
\LaTeX{} example by Uspenkiy A., group 202}
\end{center}
\lipsum[1]
$x = a + b - c$

\lipsum[2]
$$y = ab + c^5$$
\lipsum[3]
\begin{equation}
	z = \frac{a}{b} + \phi
\end{equation}
\end{document}